Logic/FirstOrder/Basic/Calculus.lean
@@ -515,6 +515,20 @@ lemma inconsistent_lMap : ¬System.Consistent T → ¬System.Consistent (T.lMap 
 
 end System
 
+namespace Theory
+
+variable (T U : Theory L)
+
+instance {L : Language} : Add (Theory L) := ⟨(· ∪ ·)⟩
+
+lemma add_def : T + U = T ∪ U := rfl
+
+instance {T U : Theory L} : T ≾ T + U := ⟨fun {f} hf ↦ System.weakening hf (by simp [add_def])⟩
+
+instance {T U : Theory L} : U ≾ T + U := ⟨fun {f} hf ↦ System.weakening hf (by simp [add_def])⟩
+
+end Theory
+
 end FirstOrder
 
 end LO
